src/compiler/core/OCL_compiler_floor1_astype.thy
@@ -135,7 +135,7 @@ definition "print_astype_lemmas_id = start_map' (\<lambda>expr.
   (let name_set = print_astype_lemma_cp_set expr in
    case name_set of [] \<Rightarrow> [] | _ \<Rightarrow> List_map Thy_lemmas_simp
   [ Lemmas_simp \<open>\<close> (List_map (\<lambda>((isub_name, _), name).
-    Thm_str (flatten [isub_name const_oclastype, \<open>_\<close>, name])) name_set) ]))"
+    Thm_thm (flatten [isub_name const_oclastype, \<open>_\<close>, name])) name_set) ]))"
 
 definition "print_astype_lemma_cp_set2 =
   (if activate_simp_optimization then
@@ -151,7 +151,7 @@ definition "print_astype_lemmas_id2 = start_map'' id o (\<lambda>expr base_attr 
   (let name_set = print_astype_lemma_cp_set2 expr base_attr in
    case name_set of [] \<Rightarrow> [] | _ \<Rightarrow> List_map Thy_lemmas_simp
   [ Lemmas_simp \<open>\<close> (List_map (\<lambda>((isub_name_h, _), (_, name)).
-    Thm_str (flatten [isub_name_h const_oclastype, \<open>_\<close>, name])) name_set) ]))"
+    Thm_thm (flatten [isub_name_h const_oclastype, \<open>_\<close>, name])) name_set) ]))"
 
 definition "print_astype_lemma_cp expr = (start_map Thy_lemma_by o get_hierarchy_map (
   let check_opt =
@@ -169,7 +169,7 @@ definition "print_astype_lemma_cp expr = (start_map Thy_lemma_by o get_hierarchy
                (Expr_annot_ocl (Expr_app var_p [Expr_annot_ocl (Expr_basic [var_x]) name3]) name2)
                (Expr_basic [dot_astype name1])))])
       []
-      (C.by [M.rule (Thm_str \<open>cpI1\<close>), if check_opt name1 name2 then M.simp
+      (C.by [M.rule (Thm_thm \<open>cpI1\<close>), if check_opt name1 name2 then M.simp
                                              else M.simp_add [flatten [const_oclastype, isub_of_str name1, \<open>_\<close>, name2]]])
   )) (\<lambda>x. (x, x, x))) expr"
 
@@ -177,7 +177,7 @@ definition "print_astype_lemmas_cp = start_map'
  (if activate_simp_optimization then List_map Thy_lemmas_simp o
   (\<lambda>expr. [Lemmas_simp \<open>\<close> (get_hierarchy_map
   (\<lambda>name1 name2 name3.
-      Thm_str (flatten [\<open>cp_\<close>, const_oclastype, isub_of_str name1, \<open>_\<close>, name3, \<open>_\<close>, name2]))
+      Thm_thm (flatten [\<open>cp_\<close>, const_oclastype, isub_of_str name1, \<open>_\<close>, name3, \<open>_\<close>, name2]))
   (\<lambda>x. (x, x, x)) expr)])
   else (\<lambda>_. []))"
 
@@ -197,7 +197,7 @@ definition "print_astype_lemma_strict expr = (start_map Thy_lemma_by o
              (Expr_basic [name2])]
       []
       (C.by (if check_opt name1 name3 then [M.simp]
-                else [M.rule (Thm_str \<open>ext\<close>)
+                else [M.rule (Thm_thm \<open>ext\<close>)
                                       , M.simp_add (flatten [const_oclastype, isub_of_str name1, \<open>_\<close>, name3]
                                                       # hol_definition \<open>bot_option\<close>
                                                       # List_map hol_definition (if name2 = \<open>invalid\<close> then [\<open>invalid\<close>]
@@ -207,7 +207,7 @@ definition "print_astype_lemma_strict expr = (start_map Thy_lemma_by o
 definition "print_astype_lemmas_strict = start_map'
  (if activate_simp_optimization then List_map Thy_lemmas_simp o
   (\<lambda>expr. [ Lemmas_simp \<open>\<close> (get_hierarchy_map (\<lambda>name1 name2 name3.
-        Thm_str (flatten [const_oclastype, isub_of_str name1, \<open>_\<close>, name3, \<open>_\<close>, name2])
+        Thm_thm (flatten [const_oclastype, isub_of_str name1, \<open>_\<close>, name3, \<open>_\<close>, name2])
       ) (\<lambda>x. (x, [\<open>invalid\<close>,\<open>null\<close>], x)) expr)])
   else (\<lambda>_. []))"
 
@@ -221,7 +221,7 @@ definition "print_astype_defined = start_m Thy_lemma_by m_class_default
           (flatten [isub_name const_oclastype, \<open>_\<close>, h_name, \<open>_defined\<close>])
           [(var_isdef, False, f (Expr_basic [var_X]))]
           (f (Expr_postunary (Expr_annot_ocl (Expr_basic [var_X]) h_name) (Expr_basic [dot_astype name])))
-          [C.using [Thm_str var_isdef]]
+          [C.using [Thm_thm var_isdef]]
           (C.by [M.auto_simp_add (flatten [isub_name const_oclastype, \<open>_\<close>, h_name]
                                         # \<open>foundation16\<close>
                                         # List_map hol_definition [\<open>null_option\<close>, \<open>bot_option\<close> ])]) ]
@@ -240,9 +240,9 @@ definition "print_astype_up_d_cast0 = start_map Thy_lemma_by o
              (let\<^sub>O\<^sub>C\<^sub>a\<^sub>m\<^sub>l asty = \<lambda>x ty. Expr_warning_parenthesis (Expr_postunary x (Expr_basic [dot_astype ty])) in
               asty (asty (Expr_annot_ocl (Expr_basic [var_X]) name_pers) name_any) name_pers)
              \<open>\<triangleq>\<close> (Expr_basic [var_X])))
-        [C.using [Thm_str var_isdef]]
+        [C.using [Thm_thm var_isdef]]
         (C.by [M.auto_simp_add_split
-                                    (List_map Thm_str
+                                    (List_map Thm_thm
                                     ( flatten [const_oclastype, isub_of_str name_any, \<open>_\<close>, name_pers]
                                     # flatten [const_oclastype, isub_of_str name_pers, \<open>_\<close>, name_any]
                                     # \<open>foundation22\<close>
@@ -263,12 +263,12 @@ definition "print_astype_up_d_cast = start_map Thy_lemma_by o
               asty (asty (Expr_annot_ocl (Expr_basic [var_X]) name_pers) name_any) name_pers)
              \<open>=\<close> (Expr_basic [var_X]))
         (List_map C.apply
-          [[M.rule (Thm_str \<open>ext\<close>), M.rename_tac [var_tau]]
-          ,[M.rule (Thm_THEN (Thm_str \<open>foundation22\<close>) (Thm_str \<open>iffD1\<close>))]
+          [[M.rule (Thm_thm \<open>ext\<close>), M.rename_tac [var_tau]]
+          ,[M.rule (Thm_THEN (Thm_thm \<open>foundation22\<close>) (Thm_thm \<open>iffD1\<close>))]
           ,[M.case_tac (Expr_binop (Expr_basic [var_tau]) \<open>\<Turnstile>\<close>
               (Expr_app \<open>\<delta>\<close> [Expr_basic [var_X]])), M.simp_add [print_astype_up_d_cast0_name name_any name_pers]]
-          ,[M.simp_add [\<open>defined_split\<close>], M.elim (Thm_str \<open>disjE\<close>)]
-          ,[M.plus' [M.erule (Thm_str \<open>StrongEq_L_subst2_rev\<close>), M.simp, M.simp]]])
+          ,[M.simp_add [\<open>defined_split\<close>], M.elim (Thm_thm \<open>disjE\<close>)]
+          ,[M.plus' [M.erule (Thm_thm \<open>StrongEq_L_subst2_rev\<close>), M.simp, M.simp]]])
         C.done)"
 
 definition "print_astype_d_up_cast = start_map Thy_lemma_by o
@@ -294,8 +294,8 @@ definition "print_astype_d_up_cast = start_map Thy_lemma_by o
                  \<open>\<doteq>\<close>
                  (b var_X))))
       (List_map C.apply
-        [[M.case_tac (f_tau not_val), M.rule (Thm_str \<open>foundation25\<close>), M.simp]])
-      (C.by [ M.rule (Thm_str \<open>foundation25'\<close>)
+        [[M.case_tac (f_tau not_val), M.rule (Thm_thm \<open>foundation25\<close>), M.simp]])
+      (C.by [ M.rule (Thm_thm \<open>foundation25'\<close>)
                , M.simp_add [ var_def_X
                               , print_astype_up_d_cast_name name_any name_pers
                               , \<open>StrictRefEq\<^sub>O\<^sub>b\<^sub>j\<^sub>e\<^sub>c\<^sub>t_sym\<close>]]) )"
@@ -320,13 +320,13 @@ definition "print_astype_lemma_const expr = (start_map Thy_lemma_by o
                    (Expr_basic [dot_astype name1]) ])
         []
         (C.by [ M.simp_add [d \<open>const\<close>]
-                 , M.option [M.metis0 [\<open>no_types\<close>] (List_map Thm_str (n # \<open>prod.collapse\<close> # List_map d [\<open>bot_option\<close>, \<open>invalid\<close>, \<open>null_fun\<close>, \<open>null_option\<close>]))]])))
+                 , M.option [M.metis0 [\<open>no_types\<close>] (List_map Thm_thm (n # \<open>prod.collapse\<close> # List_map d [\<open>bot_option\<close>, \<open>invalid\<close>, \<open>null_fun\<close>, \<open>null_option\<close>]))]])))
    (\<lambda>x. (x, [\<open>const\<close>], x))) expr"
 
 definition "print_astype_lemmas_const = start_map'
  (if activate_simp_optimization then List_map Thy_lemmas_simp o
   (\<lambda>expr. [ Lemmas_simp \<open>\<close> (get_hierarchy_map (\<lambda>name1 name2 name3.
-        Thm_str (flatten [const_oclastype, isub_of_str name1, \<open>_\<close>, name3, \<open>_\<close>, name2])
+        Thm_thm (flatten [const_oclastype, isub_of_str name1, \<open>_\<close>, name3, \<open>_\<close>, name2])
       ) (\<lambda>x. (x, [\<open>const\<close>], x)) expr)])
   else (\<lambda>_. []))"
 
